BlockAllocator implementation

disk-betree/BlockAllocator.i.dfy
@@ -1,7 +1,7 @@
 include "../lib/Bitmap.i.dfy"
 include "Bounds.i.dfy"
 
-module BlockAllocator {
+module ImplModelBlockAllocator {
   import Bitmap
   import opened Bounds
   import opened Options
@@ -71,10 +71,17 @@ module BlockAllocator {
   function MarkUsedOutstanding(bam: BlockAllocatorModel, i: int) : (bam': BlockAllocatorModel)
   requires Inv(bam)
   requires 0 <= i < NumBlocks()
+  ensures Inv(bam')
   {
-    bam
+    var bam' := bam
       .(outstanding := Bitmap.BitSet(bam.outstanding, i))
-      .(full := Bitmap.BitSet(bam.full, i))
+      .(full := Bitmap.BitSet(bam.full, i));
+
+    Bitmap.reveal_BitSet();
+    Bitmap.reveal_IsSet();
+    assert forall j | 0 <= j < |bam.ephemeral| :: j != i ==> Bitmap.IsSet(bam'.ephemeral, j) == Bitmap.IsSet(bam.ephemeral, j);
+
+    bam'
   }
 
   function InitBlockAllocator(bm: Bitmap.BitmapModel) : BlockAllocatorModel
@@ -124,7 +131,7 @@ module BlockAllocator {
       None,
       bam.frozen.value,
       bam.outstanding,
-      Bitmap.Union(bam.ephemeral, bam.frozen.value)
+      Bitmap.BitUnion(bam.ephemeral, bam.frozen.value)
     )
   }
 
@@ -149,4 +156,217 @@ module BlockAllocator {
     && (res.Some? && bam.frozen.Some? ==> !Bitmap.IsSet(bam.frozen.value, res.value))
     && (res.Some? ==> !Bitmap.IsSet(bam.persistent, res.value))
     && (res.Some? ==> !Bitmap.IsSet(bam.outstanding, res.value))
+}
+
+module ImplBlockAllocator {
+  import Bitmap
+  import opened Bounds
+  import opened Options
+  import ImplModelBlockAllocator
+  import opened NativeTypes
+
+  class BlockAllocator {
+    var ephemeral: Bitmap.Bitmap;
+    var frozen: Bitmap.Bitmap?;
+    var persistent: Bitmap.Bitmap;
+    var outstanding: Bitmap.Bitmap;
+    var full: Bitmap.Bitmap;
+
+    ghost var Repr: set<object>
+
+    protected predicate Inv()
+    reads this, Repr
+    ensures Inv() ==> this in Repr
+    {
+      && this in Repr
+      && ephemeral in Repr
+      && (frozen != null ==> frozen in Repr)
+      && persistent in Repr
+      && outstanding in Repr
+      && full in Repr
+      && Repr == {this} + ephemeral.Repr + (if frozen == null then {} else frozen.Repr) + persistent.Repr + outstanding.Repr + full.Repr
+      && {this} !! ephemeral.Repr !! (if frozen == null then {} else frozen.Repr) !! persistent.Repr !! outstanding.Repr !! full.Repr
+
+      && ephemeral.Inv()
+      && (frozen != null ==> frozen.Inv())
+      && persistent.Inv()
+      && outstanding.Inv()
+      && full.Inv()
+      && Bitmap.Len(ephemeral.I()) == NumBlocks()
+      && (frozen != null ==> Bitmap.Len(frozen.I()) == NumBlocks())
+      && Bitmap.Len(persistent.I()) == NumBlocks()
+      && Bitmap.Len(outstanding.I()) == NumBlocks()
+      && Bitmap.Len(full.I()) == NumBlocks()
+    }
+
+    protected function I() : ImplModelBlockAllocator.BlockAllocatorModel
+    reads this, Repr
+    requires Inv()
+    {
+      ImplModelBlockAllocator.BlockAllocatorModel(ephemeral.I(),
+          (if frozen == null then None else Some(frozen.I())),
+          persistent.I(),
+          outstanding.I(),
+          full.I())
+    }
+
+    constructor(bm: Bitmap.Bitmap)
+    requires bm.Inv()
+    requires Bitmap.Len(bm.I()) == NumBlocks()
+    ensures Inv()
+    ensures forall o | o in Repr :: fresh(o) || o in bm.Repr
+    ensures I() == ImplModelBlockAllocator.InitBlockAllocator(bm.I())
+    {
+      ephemeral := bm;
+      frozen := null;
+      persistent := new Bitmap.Bitmap.Clone(bm);
+      outstanding := new Bitmap.Bitmap(NumBlocksUint64());
+      full := new Bitmap.Bitmap.Clone(bm);
+
+      new;
+
+      Repr := {this} + ephemeral.Repr + (if frozen == null then {} else frozen.Repr) + persistent.Repr + outstanding.Repr + full.Repr;
+    }
+
+    method Alloc() returns (res : Option<int>)
+    requires Inv()
+    ensures res == ImplModelBlockAllocator.Alloc(I())
+    {
+      res := full.Alloc();
+    }
+
+    method MarkUsedEphemeral(i: uint64)
+    requires Inv()
+    requires ImplModelBlockAllocator.Inv(I())
+    requires i as int < NumBlocks()
+    modifies Repr
+    ensures Inv()
+    ensures Repr == old(Repr)
+    ensures I() == ImplModelBlockAllocator.MarkUsedEphemeral(old(I()), i as int)
+    {
+      ephemeral.Set(i);
+      full.Set(i);
+    }
+
+    method MarkUsedFrozen(i: uint64)
+    requires Inv()
+    requires ImplModelBlockAllocator.Inv(I())
+    requires i as int < NumBlocks()
+    requires I().frozen.Some?
+    modifies Repr
+    ensures Inv()
+    ensures Repr == old(Repr)
+    ensures I() == ImplModelBlockAllocator.MarkUsedFrozen(old(I()), i as int)
+    {
+      frozen.Set(i);
+      full.Set(i);
+    }
+
+    method MarkUsedOutstanding(i: uint64)
+    requires Inv()
+    requires ImplModelBlockAllocator.Inv(I())
+    requires i as int < NumBlocks()
+    modifies Repr
+    ensures Inv()
+    ensures Repr == old(Repr)
+    ensures I() == ImplModelBlockAllocator.MarkUsedOutstanding(old(I()), i as int)
+    {
+      outstanding.Set(i);
+      full.Set(i);
+    }
+
+    method MarkFreeOutstanding(i: uint64)
+    requires Inv()
+    requires ImplModelBlockAllocator.Inv(I())
+    requires i as int < NumBlocks()
+    modifies Repr
+    ensures Inv()
+    ensures Repr == old(Repr)
+    ensures I() == ImplModelBlockAllocator.MarkFreeOutstanding(old(I()), i as int)
+    {
+      outstanding.Unset(i);
+
+      var b0 := false;
+      if frozen != null {
+        b0 := frozen.GetIsSet(i);
+      }
+      if !b0 {
+        var b1 := ephemeral.GetIsSet(i);
+        if !b1 {
+          var b2 := persistent.GetIsSet(i);
+          if !b2 {
+            full.Unset(i);
+          }
+        }
+      }
+
+      Bitmap.reveal_BitUnset();
+      Bitmap.reveal_IsSet();
+
+      assert Inv();
+    }
+
+    method MarkFreeEphemeral(i: uint64)
+    requires Inv()
+    requires ImplModelBlockAllocator.Inv(I())
+    requires i as int < NumBlocks()
+    modifies Repr
+    ensures Inv()
+    ensures Repr == old(Repr)
+    ensures I() == ImplModelBlockAllocator.MarkFreeEphemeral(old(I()), i as int)
+    {
+      ephemeral.Unset(i);
+
+      var b0 := false;
+      if frozen != null {
+        b0 := frozen.GetIsSet(i);
+      }
+      if !b0 {
+        var b1 := outstanding.GetIsSet(i);
+        if !b1 {
+          var b2 := persistent.GetIsSet(i);
+          if !b2 {
+            full.Unset(i);
+          }
+        }
+      }
+
+      Bitmap.reveal_BitUnset();
+      Bitmap.reveal_IsSet();
+
+      assert forall j | 0 <= j < |ephemeral.I()| :: j != i as int ==> Bitmap.IsSet(ephemeral.I(), j) == Bitmap.IsSet(old(ephemeral.I()), j);
+
+      assert Inv();
+    }
+
+    method MoveFrozenToPersistent()
+    requires Inv()
+    requires ImplModelBlockAllocator.Inv(I())
+    requires I().frozen.Some?
+    modifies Repr
+    ensures Inv()
+    ensures forall o | o in Repr :: o in old(Repr) || fresh(o)
+    ensures I() == ImplModelBlockAllocator.MoveFrozenToPersistent(old(I()))
+    {
+      persistent := frozen;
+      frozen := null;
+      full := new Bitmap.Bitmap.Union(ephemeral, persistent);
+
+      Repr := {this} + ephemeral.Repr + (if frozen == null then {} else frozen.Repr) + persistent.Repr + outstanding.Repr + full.Repr;
+    }
+
+    method CopyEphemeralToFrozen()
+    requires Inv()
+    requires ImplModelBlockAllocator.Inv(I())
+    modifies Repr
+    ensures Inv()
+    ensures forall o | o in Repr :: o in old(Repr) || fresh(o)
+    ensures I() == ImplModelBlockAllocator.CopyEphemeralToFrozen(old(I()))
+    {
+      frozen := new Bitmap.Bitmap.Clone(ephemeral);
+
+      Repr := {this} + ephemeral.Repr + (if frozen == null then {} else frozen.Repr) + persistent.Repr + outstanding.Repr + full.Repr;
+    }
+
+  }
 }
